pulse/examples/dsls/mini_steel/Pulse.Soundness.Exists.fst
@@ -3,3 +3,4 @@ module Pulse.Soundness.Exists
 let exists_inversion _ = admit ()
 let elim_exists_soundness _ _ = admit ()
 let intro_exists_soundness _ _ _ = admit ()
+let intro_exists_erased_soundness _ _ _ = admit ()
